\chapter{The Baker-Campbell-Hausdorf Formula\label{ch:bchf}}
The Baker-Campbell-Hausdorf formula for a complex number $\lambda$ and operators $A,G$ and $C_n$ is given by
\beq
\label{eq:bchf}
e^{\lambda G}Ae^{-\lambda G} = \sum\limits_{n = 0}^\infty \frac{\lambda^n}{n!} C_n
\eeq
where $C_n$ is defined recursively such that $C_0 = A$ and $C_n = [G,C_{n-1}]$. Several references on Lie Algebras such as \cite{liealgs}, \cite{liealgs2} and \cite{liealgs3} provide interesting proofs of the formula.

Here, we are interested in applying the Baker-Campbell-Hausdorf formula to the unitary matrix which represents the operation of an optical beamsplitter. In particular, for a beamsplitter $B$ of angle $\theta$, the unitary matrix representation is
\beq
\label{eq:bseq}
B = \exp{\theta(\adj{a} b - a\adj{b})}
\eeq
For such a beamsplitter, we will compute $Ba\adj{B}$ and $Bb\adj{B}$ for annihilation operators $a$ and $b$ and creation operators $\adj{a}$ and $\adj{b}$. Recall from \ref{annihilators} that for annihilation operators $\alpha$ and $\beta$, $[\alpha,\adj{\alpha}] = [\beta,\adj{\beta}] = 1$ and $[\alpha,\beta] = [\adj{\alpha},\beta] = [\alpha,\adj{\beta}] = [\adj{\alpha},\adj{\beta}] = 0$. 
Setting $G$ in \eqref{eq:bchf} to $\adj{a} b - a\adj{b}$, we have
\begin{align*}
[G,a] &= (\adj{a} b - a\adj{b})a - a(\adj{a} b - a\adj{b}) \\
&= \adj{a}ba - a\adj{b}a - a\adj{a}b + aa\adj{b}\\
&= \adj{a}ba - a\adj{a}b + aa\adj{b} - a\adj{b}a\\
&= [\adj{a}b,a] + a\cancelto{0}{[a,\adj{b}]}\\
&= [\adj{a}b,a]\\
&= \adj{a}ba - \adj{a}ab + \adj{a}ab - a\adj{a}b\\
&= \adj{a}\cancelto{0}{[b,a]} - [a,\adj{a}]b\\
&= -b
\end{align*}
Similarly, we can prove that $[G,b] = a$. We summarize these results below. 
\begin{align}
\label{eq:Gcommutes}
[G,a] &= -b\\
[G,b] &= a
\end{align}
We can now generalize the terms of $C_n$. Setting $C_0 = a$, $C_1 = [G,a] = -b$, $C_2 = [G,C_1] = -a$, $C_3 = [G,C_2] = b,\ldots$ and generally,
\begin{align*}
C_n &= i^na \text{ for even n}\\
C_n &= i^{n+1}b \text{ for odd n}
\end{align*}
Hence,
\begin{align}
Ba\adj{B} &= e^{\theta G}ae^{-\theta G}\\
&= \sum\limits_{n=0}^\infty \frac{\theta^n}{n!}C_n\\
&= \sum\limits_{n = even} \frac{(i\theta)^n}{n!}a + i\sum\limits_{n = odd}^\infty \frac{(i\theta)^n}{n!}b\\
&= a\cos\theta + b\sin\theta
\end{align}
Similarly, $Bb\adj{B} = -a\sin\theta + b\cos\theta$.$\qed$
