\chapter{Exponentiating Matrices\label{ch:expmtx}}

In this appendix, we prove the following.
\beq
\exp{iAx} = cos(x)I + isin(x)A
\eeq
for a real number $x$ and matrix $A$ such that $A^2 = I$ and $A^0 = I$. Recall the power series expansion for the exponential $\exp{x}$ for all $x$.

\beq
\exp{x} = \sum\limits_{n=0}^{\infty} \frac{x^n}{n!}
\eeq
We now rewrite this power series expansion for $\exp{x}$ after replacing $x$ by $iAx$.

\begin{align}
\exp{iAx} &= \sum\limits_{n=0}^{\infty}\frac{\left(iAx\right)^n}{n!}\\
&= \frac{I}{0!} + \frac{iAx}{1!} + \frac{\left(iAx\right)^2}{2!} + \frac{\left(iAx\right)^3}{3!} + \ldots\\
&= \frac{A^2}{0!} + \frac{iAx}{1!} + \frac{\left(iAx\right)^2}{2!} + \frac{\left(iAx\right)^3}{3!} + \ldots
\end{align}
Noting that even powers of $A$ reduce to identity and $i^2 = -1$, we now rearrange the terms in the above equation as follows.

\begin{align}
\exp{iAx} &= \frac{A^2}{0!} + \frac{iAx}{1!} + \frac{\left(iAx\right)^2}{2!} + \frac{\left(iAx\right)^3}{3!} + \ldots\\
&= \left(\frac{x^0}{0!} - \frac{x^2}{2!} + \frac{x^4}{4!} - \ldots \right)I + i\left(\frac{x^1}{1!} - \frac{x^3}{3!} + \frac{x^5}{5!} - \ldots \right)A\\
\end{align}
The power series expansions for the sine and cosine functions appear in the above equation. We will state the power series expansions for these two functions below.

\begin{align}
sin(x) &= \sum\limits_{n=0}^{\infty} \left(-1\right)^n\frac{x^{2n+1}}{\left(2n+1\right)!} = \left(\frac{x^1}{1!} - \frac{x^3}{3!} + \frac{x^5}{5!} - \ldots \right)\\
cos(x) &= \sum\limits_{n=0}^{\infty} \left(-1\right)^n\frac{x^{2n}}{\left(2n\right)!} = \left(\frac{x^0}{0!} - \frac{x^2}{2!} + \frac{x^4}{4!} - \ldots \right)
\end{align}
Therefore,

\begin{align}
\exp{iAx} &= \left(\frac{x^0}{0!} - \frac{x^2}{2!} + \frac{x^4}{4!} - \ldots \right)I + i\left(\frac{x^1}{1!} - \frac{x^3}{3!} + \frac{x^5}{5!} - \ldots \right)A\\
&= cos(x)I + isin(x)A\qed
\end{align}
